code/ecdsap256/Hacl.Impl.P256.Scalar.fsti
@@ -12,6 +12,7 @@ open Hacl.Impl.P256.Bignum
 
 module S = Spec.P256
 module SM = Hacl.Spec.P256.Montgomery
+module BSeq = Lib.ByteSequence
 
 #set-options "--z3rlimit 30 --fuel 0 --ifuel 0"
 
@@ -38,6 +39,17 @@ val bn_is_lt_order_and_gt_zero_mask4: f:felem -> Stack uint64
   (requires fun h -> live h f)
   (ensures  fun h0 r h1 -> modifies0 h0 h1 /\
     (if 0 < as_nat h0 f && as_nat h0 f < S.order then v r = ones_v U64 else v r = 0))
+
+
+inline_for_extraction noextract
+val load_qelem_conditional: res:felem -> b:lbuffer uint8 32ul -> Stack uint64
+  (requires fun h ->
+    live h res /\ live h b /\ disjoint res b)
+  (ensures fun h0 m h1 -> modifies (loc res) h0 h1 /\
+   (let b_nat = BSeq.nat_from_bytes_be (as_seq h0 b) in
+    let is_b_valid = 0 < b_nat && b_nat < S.order in
+    (v m = ones_v U64 \/ v m = 0) /\ (v m = ones_v U64) = is_b_valid /\
+    as_nat h1 res == (if is_b_valid then b_nat else 1)))
 
 
 ///  Field Arithmetic
