code/ecdsap256/Hacl.Impl.P256.Point.fsti
@@ -9,12 +9,10 @@ open Lib.Buffer
 
 open Hacl.Impl.P256.Bignum
 
-module LSeq = Lib.Sequence
-module BSeq = Lib.ByteSequence
-
 module S = Spec.P256
 module SB = Hacl.Spec.P256.Bignum
 module SM = Hacl.Spec.P256.Montgomery
+module LSeq = Lib.Sequence
 
 #set-options "--z3rlimit 30 --fuel 0 --ifuel 0"
 
